Move over code from [DListRef] to [DListLow]

DListLow.fst
@@ -1,20 +1,10 @@
 module DListLow
 
 open FStar
-open FStar.HyperStack
 open FStar.HyperStack.ST
-open FStar.Buffer
-open FStar.Int
 open FStar.Ghost
 open FStar.Seq
 open Gpointers
-module U64 = FStar.UInt64
-module U32 = FStar.UInt32
-module U16 = FStar.UInt16
-module U8 = FStar.UInt8
-module HS = FStar.HyperStack
-module B = FStar.Buffer
-module ST = FStar.HyperStack.ST
 
 unopteq
 (** Node of a doubly linked list *)
@@ -45,44 +35,16 @@ val empty_list: #t:Type -> dlisthead t
 let empty_list #t =
   { lhead = null ; ltail = null ; nodes = hide createEmpty }
 
-val getSome: (a:gpointer_or_null 'a{is_not_null a}) -> (b:gpointer 'a{g_ptr_eq a b})
-let getSome a = a
-
-unfold let (@) (a:gpointer 't) (h0:HS.mem{h0 `B.live` a}) = B.get h0 a 0
-unfold let (^@) (a:gpointer_or_null 't{is_not_null a}) (h0:HS.mem{h0 `B.live` (getSome a)}) = (getSome a) @ h0
-
 unfold let (.[]) (s:seq 'a) (n:nat{n < length s}) = index s n
 
-// logic : Cannot use due to https://github.com/FStarLang/FStar/issues/638
-let not_aliased (#t:Type) (a:gpointer_or_null t) (b:gpointer_or_null t) : GTot Type0 =
-  is_null a \/ is_null b \/
-  (let (a:_{is_not_null a}) = a in // workaround for not using two phase type checker
-   let (b:_{is_not_null b}) = b in
-   disjoint (getSome a) (getSome b))
-
-// logic : Cannot use due to https://github.com/FStarLang/FStar/issues/638
-let not_aliased0 (#t:Type) (a:gpointer t) (b:gpointer_or_null t) : GTot Type0 =
-  is_null b \/
-  (let (b:_{is_not_null b}) = b in // workaround for not using two phase type checker
-   disjoint a (getSome b))
-
 logic
-let not_aliased00 (#t:Type) (a:gpointer t) (b:gpointer t) : GTot Type0 =
-  disjoint a b
-
-logic
-let dlist_is_valid' (#t:Type) (h0:HS.mem) (n:dlist t) : GTot Type0 =
+let dlist_is_valid' (#t:Type) (h0:heap) (n:dlist t) : GTot Type0 =
   not_aliased n.flink n.blink
 
 // logic
-let dlist_is_valid (#t:Type) (h0:HS.mem) (n:gpointer (dlist t)) : GTot Type0 =
-  h0 `B.live` n /\
+let dlist_is_valid (#t:Type) (h0:heap) (n:gpointer (dlist t)) : GTot Type0 =
+  h0 `contains` n /\
   dlist_is_valid' h0 (n@h0)
-
-let (==$) (#t:Type) (a:gpointer_or_null t) (b:gpointer t) =
-  is_not_null a /\
-  (let (a:_{is_not_null a}) = a in // workaround for not using two phase type checker
-   g_ptr_eq (getSome a) b)
 
 logic
 let ( |> ) (#t:Type) (a:dlist t) (b:gpointer (dlist t)) : GTot Type0 =
@@ -95,7 +57,7 @@ let ( <| ) (#t:Type) (a:gpointer (dlist t)) (b: dlist t) : GTot Type0 =
 irreducible
 let ( =|> ) (#t:Type) (a:gpointer (dlist t)) (b:gpointer (dlist t)) : ST unit
     (requires (fun h0 ->
-         h0 `B.live` a /\ h0 `B.live` b /\
+         h0 `contains` a /\ h0 `contains` b /\
          not_aliased00 a b /\
          not_aliased0 b (a@h0).blink))
     (ensures (fun h1 _ h2 ->
@@ -105,12 +67,12 @@ let ( =|> ) (#t:Type) (a:gpointer (dlist t)) (b:gpointer (dlist t)) : ST unit
          (a@h1).blink == (a@h2).blink /\
          b@h1 == b@h2 /\
          (a@h2) |> b)) =
-  a := { !a with flink = b }
+  a := { !a with flink = of_non_null b }
 
 irreducible
 let ( <|= ) (#t:Type) (a:gpointer (dlist t)) (b:gpointer (dlist t)) : ST unit
     (requires (fun h0 ->
-         h0 `B.live` a /\ h0 `B.live` b /\
+         h0 `contains` a /\ h0 `contains` b /\
          not_aliased00 a b /\
          not_aliased0 a (b@h0).flink))
     (ensures (fun h1 _ h2 ->
@@ -120,11 +82,11 @@ let ( <|= ) (#t:Type) (a:gpointer (dlist t)) (b:gpointer (dlist t)) : ST unit
          (b@h1).p == (b@h2).p /\
          (b@h1).flink == (b@h2).flink /\
          a <| (b@h2))) =
-  b := { !b with blink = a }
+  b := { !b with blink = of_non_null a }
 
 irreducible
 let ( !=|> ) (#t:Type) (a:gpointer (dlist t)) : ST unit
-    (requires (fun h0 -> h0 `B.live` a))
+    (requires (fun h0 -> h0 `contains` a))
     (ensures (fun h1 _ h2 ->
          modifies_1 a h1 h2 /\
          dlist_is_valid h2 a /\
@@ -135,7 +97,7 @@ let ( !=|> ) (#t:Type) (a:gpointer (dlist t)) : ST unit
 
 irreducible
 let ( !<|= ) (#t:Type) (a:gpointer (dlist t)) : ST unit
-    (requires (fun h0 -> h0 `B.live` a))
+    (requires (fun h0 -> h0 `contains` a))
     (ensures (fun h1 _ h2 ->
          modifies_1 a h1 h2 /\
          dlist_is_valid h2 a /\
@@ -149,15 +111,15 @@ unfold let (^+) (#t:Type) (a:t) (b:erased (seq t)) : Tot (erased (seq t)) = elif
 unfold let (+^) (#t:Type) (a:erased (seq t)) (b:t) : Tot (erased (seq t)) = elift2 Seq.snoc a (hide b)
 
 logic
-let all_nodes_contained (#t:Type) (h0:HS.mem) (h:dlisthead t) : GTot Type0 =
+let all_nodes_contained (#t:Type) (h0:heap) (h:dlisthead t) : GTot Type0 =
   let nodes = reveal h.nodes in
-  (is_not_null h.lhead ==> h0 `B.live` (getSome h.lhead)) /\
-  (is_not_null h.ltail ==> h0 `B.live` (getSome h.ltail)) /\
-  (forall i. {:pattern (h0 `B.live` nodes.[i])}
-     h0 `B.live` nodes.[i])
+  (is_not_null h.lhead ==> h0 `contains` (non_null h.lhead)) /\
+  (is_not_null h.ltail ==> h0 `contains` (non_null h.ltail)) /\
+  (forall i. {:pattern (h0 `contains` nodes.[i])}
+     h0 `contains` nodes.[i])
 
 logic
-let flink_valid (#t:Type) (h0:HS.mem) (h:dlisthead t) : GTot Type0 =
+let flink_valid (#t:Type) (h0:heap) (h:dlisthead t) : GTot Type0 =
   let nodes = reveal h.nodes in
   let len = length nodes in
   all_nodes_contained h0 h /\
@@ -166,7 +128,7 @@ let flink_valid (#t:Type) (h0:HS.mem) (h:dlisthead t) : GTot Type0 =
       nodes.[i]@h0 |> nodes.[i+1]))
 
 logic
-let blink_valid (#t:Type) (h0:HS.mem) (h:dlisthead t) : GTot Type0 =
+let blink_valid (#t:Type) (h0:heap) (h:dlisthead t) : GTot Type0 =
   let nodes = reveal h.nodes in
   let len = length nodes in
   all_nodes_contained h0 h /\
@@ -175,7 +137,7 @@ let blink_valid (#t:Type) (h0:HS.mem) (h:dlisthead t) : GTot Type0 =
       nodes.[i-1] <| nodes.[i]@h0))
 
 logic
-let dlisthead_ghostly_connections (#t:Type) (h0:HS.mem) (h:dlisthead t) : GTot Type0 =
+let dlisthead_ghostly_connections (#t:Type) (h0:heap) (h:dlisthead t) : GTot Type0 =
   let nodes = reveal h.nodes in
   let len = length nodes in
   let empty = (len = 0) in
@@ -187,7 +149,7 @@ let dlisthead_ghostly_connections (#t:Type) (h0:HS.mem) (h:dlisthead t) : GTot T
     is_null (h.ltail^@h0).flink)
 
 logic
-let elements_dont_alias1 (#t:Type) (h0:HS.mem) (h:dlisthead t) : GTot Type0 =
+let elements_dont_alias1 (#t:Type) (h0:heap) (h:dlisthead t) : GTot Type0 =
   let nodes = reveal h.nodes in
   all_nodes_contained h0 h /\
   (forall i j. {:pattern (not_aliased (nodes.[i]@h0).flink (nodes.[j]@h0).flink)}
@@ -195,7 +157,7 @@ let elements_dont_alias1 (#t:Type) (h0:HS.mem) (h:dlisthead t) : GTot Type0 =
    not_aliased (nodes.[i]@h0).flink (nodes.[j]@h0).flink)
 
 logic
-let elements_dont_alias2 (#t:Type) (h0:HS.mem) (h:dlisthead t) : GTot Type0 =
+let elements_dont_alias2 (#t:Type) (h0:heap) (h:dlisthead t) : GTot Type0 =
   let nodes = reveal h.nodes in
   all_nodes_contained h0 h /\
   (forall i j. {:pattern (not_aliased (nodes.[i]@h0).blink (nodes.[j]@h0).blink)}
@@ -203,19 +165,19 @@ let elements_dont_alias2 (#t:Type) (h0:HS.mem) (h:dlisthead t) : GTot Type0 =
    not_aliased (nodes.[i]@h0).blink (nodes.[j]@h0).blink)
 
 // logic : Cannot use due to https://github.com/FStarLang/FStar/issues/638
-let elements_dont_alias (#t:Type) (h0:HS.mem) (h:dlisthead t) : GTot Type0 =
+let elements_dont_alias (#t:Type) (h0:heap) (h:dlisthead t) : GTot Type0 =
   elements_dont_alias1 h0 h /\
   elements_dont_alias2 h0 h
 
 logic
-let elements_are_valid (#t:Type) (h0:HS.mem) (h:dlisthead t) : GTot Type0 =
+let elements_are_valid (#t:Type) (h0:heap) (h:dlisthead t) : GTot Type0 =
   let nodes = reveal h.nodes in
   all_nodes_contained h0 h /\
   (forall i. {:pattern (nodes.[i])}
      dlist_is_valid h0 nodes.[i])
 
 logic
-let all_elements_distinct (#t:Type) (h0:HS.mem) (h:dlisthead t) : GTot Type0 =
+let all_elements_distinct (#t:Type) (h0:heap) (h:dlisthead t) : GTot Type0 =
     let nodes = reveal h.nodes in
     (forall i j. {:pattern (disjoint nodes.[i] nodes.[j])}
        (0 <= i /\ i < j /\ j < Seq.length nodes) ==>
@@ -224,7 +186,7 @@ let all_elements_distinct (#t:Type) (h0:HS.mem) (h:dlisthead t) : GTot Type0 =
         disjoint nodes.[i] nodes.[j]))
 
 unfold logic
-let dlisthead_is_valid (#t:Type) (h0:HS.mem) (h:dlisthead t) : GTot Type0 =
+let dlisthead_is_valid (#t:Type) (h0:heap) (h:dlisthead t) : GTot Type0 =
   let nodes = reveal h.nodes in
   let len = length nodes in
   let empty = (len = 0) in
@@ -235,14 +197,11 @@ let dlisthead_is_valid (#t:Type) (h0:HS.mem) (h:dlisthead t) : GTot Type0 =
   elements_are_valid h0 h /\
   elements_dont_alias h0 h
 
-let rec two_elements_distinct (#t:Type) (h0:HS.mem) (h:dlisthead t) (i j:int) : Lemma
+let rec two_elements_distinct (#t:Type) (h0:heap) (h:dlisthead t) (i j:int) : Lemma
   (requires (0 <= i /\ i < j /\ j < Seq.length (reveal h.nodes)) /\
-	    ~(length (reveal h.nodes) == 0) /\
             dlisthead_ghostly_connections h0 h /\
-            flink_valid h0 h /\
             blink_valid h0 h /\
-	    elements_are_valid h0 h /\
-	    elements_dont_alias h0 h)
+            elements_are_valid h0 h)
   (ensures
      (let nodes = reveal h.nodes in
       let (i:nat{i < Seq.length nodes}) = i in // workaround for not using two phase type checker
@@ -253,15 +212,15 @@ let rec two_elements_distinct (#t:Type) (h0:HS.mem) (h:dlisthead t) (i j:int) : 
     let b = FStar.StrongExcludedMiddle.strong_excluded_middle (disjoint nodes.[i] nodes.[j]) in
     if not b then (
       if i = 0 then (
-	assert( is_null (nodes.[i]@h0).blink);
+        assert( is_null (nodes.[i]@h0).blink);
         assert( is_not_null (nodes.[j]@h0).blink)
       ) else (
-	two_elements_distinct h0 h (i - 1) (j - 1)
+        two_elements_distinct h0 h (i - 1) (j - 1)
       )
     ) else ()
   ) else ()
 
-let lemma_all_elements_distinct (#t:Type) (h0:HS.mem) (h:dlisthead t) : Lemma
+let lemma_all_elements_distinct (#t:Type) (h0:heap) (h:dlisthead t) : Lemma
     (requires dlisthead_is_valid h0 h)
     (ensures all_elements_distinct h0 h) =
   let nodes = reveal h.nodes in
@@ -279,29 +238,27 @@ let lemma_all_elements_distinct (#t:Type) (h0:HS.mem) (h:dlisthead t) : Lemma
 
 let test1 () : Tot unit = assert (forall h0 t. dlisthead_is_valid h0 (empty_list #t))
 
-#set-options "--z3rlimit 100"
-
 val singletonlist: #t:eqtype -> e:gpointer (dlist t) ->
   ST (dlisthead t)
-  (requires (fun h0 -> h0 `B.live` e))
+  (requires (fun h0 -> h0 `contains` e))
   (ensures (fun h0 y h1 -> modifies_1 e h0 h1 /\ dlisthead_is_valid h1 y))
 let singletonlist #t e =
   !<|= e; !=|> e;
-  { lhead = e ; ltail = e ; nodes = ~. e }
+  { lhead = of_non_null e ; ltail = of_non_null e ; nodes = ~. e }
 
 // logic
 let contains_by_addr (#t:Type) (s:seq (gpointer t)) (x:gpointer t) : GTot Type0 =
   (exists i. g_ptr_eq s.[i] x)
 
 logic
-let member_of (#t:eqtype) (h0:HS.mem) (h:dlisthead t) (e:gpointer (dlist t)) : GTot Type0 =
+let member_of (#t:eqtype) (h0:heap) (h:dlisthead t) (e:gpointer (dlist t)) : GTot Type0 =
   let nodes = reveal h.nodes in
   nodes `contains_by_addr` e
 
 // logic : Cannot use due to https://github.com/FStarLang/FStar/issues/638
-let has_nothing_in (#t:eqtype) (h0:HS.mem)
+let has_nothing_in (#t:eqtype) (h0:heap)
     (h:dlisthead t{dlisthead_is_valid h0 h})
-    (e:gpointer (dlist t){h0 `B.live` e})
+    (e:gpointer (dlist t){h0 `contains` e})
   : GTot Type0 =
   (~(member_of h0 h e)) /\
   (not_aliased0 e h.lhead) /\
@@ -321,21 +278,27 @@ type nonempty_dlisthead t = (h:dlisthead t{is_not_null h.lhead /\ is_not_null h.
 val dlisthead_make_valid_singleton: #t:eqtype -> h:nonempty_dlisthead t ->
   ST (dlisthead t)
     (requires (fun h0 ->
-         h0 `B.live` (getSome h.lhead) /\
+         h0 `contains` (non_null h.lhead) /\
          is_null (h.lhead^@h0).flink /\ is_null (h.lhead^@h0).blink))
     (ensures (fun h1 y h2 -> modifies_none h1 h2 /\ dlisthead_is_valid h2 y))
 let dlisthead_make_valid_singleton #t h =
-  let e = h.lhead in
+  let e = non_null h.lhead in
   { h with ltail = h.lhead ; nodes = ~. e }
 
-let is_singleton (#t:Type) (h:nonempty_dlisthead t) : GTot Type0 =
-  g_ptr_eq (getSome h.lhead) (getSome h.ltail)
+let g_is_singleton (#t:Type) (h:nonempty_dlisthead t) : GTot Type0 =
+  g_ptr_eq (non_null h.lhead) (non_null h.ltail)
+
+let is_singleton (#t:Type) (h:nonempty_dlisthead t) :
+  ST bool
+    (requires (fun h0 -> h0 `contains` (non_null h.lhead) /\ h0 `contains` (non_null h.ltail)))
+    (ensures (fun h0 b h1 -> h0==h1 /\ (b <==> g_is_singleton h))) =
+  ptr_eq (non_null h.lhead) (non_null h.ltail)
 
 val nonempty_singleton_properties :
   #t:Type ->
   h:nonempty_dlisthead t ->
   ST unit
-    (requires (fun h0 -> dlisthead_is_valid h0 h /\ is_singleton h))
+    (requires (fun h0 -> dlisthead_is_valid h0 h /\ g_is_singleton h))
     (ensures (fun h0 _ h1 -> h0 == h1 /\ Seq.length (reveal h.nodes) == 1))
 let nonempty_singleton_properties #t h = ()
 
@@ -343,7 +306,7 @@ val nonempty_nonsingleton_properties :
   #t:Type ->
   h:nonempty_dlisthead t ->
   ST unit
-    (requires (fun h0 -> dlisthead_is_valid h0 h /\ ~(g_ptr_eq (getSome h.lhead) (getSome h.ltail))))
+    (requires (fun h0 -> dlisthead_is_valid h0 h /\ ~(g_is_singleton h)))
     (ensures (fun h0 _ h1 -> h0 == h1 /\ Seq.length (reveal h.nodes) > 1))
 let nonempty_nonsingleton_properties #t h = ()
 
@@ -353,18 +316,18 @@ val ghost_append_properties: #t:Type -> a:t -> b:erased (seq t) ->
            j = i + 1 /\ 0 <= i /\ i < length (reveal b) ==> (reveal b).[i] == (reveal r).[j])
 let ghost_append_properties #t a b = ()
 
-#set-options "--z3rlimit 300 --z3refresh"
+#set-options "--z3rlimit 100 --z3refresh"
 
 val dlisthead_update_head: #t:eqtype -> h:nonempty_dlisthead t -> e:gpointer (dlist t) ->
   ST (dlisthead t)
     (requires (fun h0 -> dlisthead_is_valid h0 h /\ dlist_is_valid h0 e /\ has_nothing_in h0 h e))
-    (ensures (fun h1 y h2 -> modifies_2 e (getSome h.lhead) h1 h2 /\ dlisthead_is_valid h2 y))
+    (ensures (fun h1 y h2 -> modifies_2 e (non_null h.lhead) h1 h2 /\ dlisthead_is_valid h2 y))
 let dlisthead_update_head (#t:eqtype) (h:nonempty_dlisthead t) (e:gpointer (dlist t)) =
-  let n = h.lhead in
+  let n = non_null h.lhead in
   !<|= e;
   e =|> n;
   e <|= n;
-  { lhead = e ; ltail = h.ltail ; nodes = e ^+ h.nodes }
+  { lhead = of_non_null e ; ltail = h.ltail ; nodes = e ^+ h.nodes }
 
 #reset-options
 
@@ -373,7 +336,7 @@ val insertHeadList : #t:eqtype -> h:dlisthead t -> e:gpointer (dlist t) ->
     (requires (fun h0 -> dlisthead_is_valid h0 h /\ dlist_is_valid h0 e /\ has_nothing_in h0 h e))
     (ensures (fun h1 y h2 ->
          (is_not_null h.lhead ==>
-          modifies_2 e (getSome h.lhead) h1 h2) /\
+          modifies_2 e (non_null h.lhead) h1 h2) /\
          (~(is_not_null h.lhead) ==>
           modifies_1 e h1 h2) /\
          dlisthead_is_valid h2 y))
@@ -382,19 +345,19 @@ let insertHeadList #t h e =
   then dlisthead_update_head h e
   else singletonlist e
 
-#set-options "--z3rlimit 300 --z3refresh"
+#set-options "--z3rlimit 100 --z3refresh"
 
 val dlisthead_update_tail: #t:eqtype -> h:nonempty_dlisthead t -> e:gpointer (dlist t) ->
   ST (dlisthead t)
     (requires (fun h0 -> dlisthead_is_valid h0 h /\ dlist_is_valid h0 e /\ has_nothing_in h0 h e))
-    (ensures (fun h1 y h2 -> modifies_2 e (getSome h.ltail) h1 h2 /\ dlisthead_is_valid h2 y))
+    (ensures (fun h1 y h2 -> modifies_2 e (non_null h.ltail) h1 h2 /\ dlisthead_is_valid h2 y))
 let dlisthead_update_tail #t h e =
   let previously_singleton = is_singleton h in
-  let n = h.ltail in
+  let n = non_null h.ltail in
   !=|> e;
   n =|> e;
   n <|= e;
-  { lhead = h.lhead ; ltail = e ; nodes = h.nodes +^ e }
+  { lhead = h.lhead ; ltail = of_non_null e ; nodes = h.nodes +^ e }
 
 #reset-options
 
@@ -403,7 +366,7 @@ val insertTailList : #t:eqtype -> h:dlisthead t -> e:gpointer (dlist t) ->
     (requires (fun h0 -> dlisthead_is_valid h0 h /\ dlist_is_valid h0 e /\ has_nothing_in h0 h e))
     (ensures (fun h1 y h2 ->
          (is_not_null h.ltail ==>
-          modifies_2 e (getSome h.ltail) h1 h2) /\
+          modifies_2 e (non_null h.ltail) h1 h2) /\
          (~(is_not_null h.lhead) ==>
           modifies_1 e h1 h2) /\
          dlisthead_is_valid h2 y))
@@ -415,29 +378,29 @@ let insertTailList #t h e =
 unfold let ghost_tail (#t:Type) (s:erased (seq t){Seq.length (reveal s) > 0}) : Tot (erased (seq t)) =
   hide (Seq.tail (reveal s))
 
-#set-options "--z3rlimit 300"
+#set-options "--z3rlimit 100"
 
 val dlisthead_remove_head: #t:eqtype -> h:nonempty_dlisthead t ->
   ST (dlisthead t)
     (requires (fun h0 -> dlisthead_is_valid h0 h))
     (ensures (fun h1 y h2 ->
-          modifies_1 (getSome h.lhead) h1 h2) /\
-          modifies_2 (getSome h.lhead) (reveal h.nodes).[1] h1 h2) /\
-         (is_singleton h ==>
-         (~(is_singleton h) ==>
+         (g_is_singleton h ==>
+          modifies_1 (non_null h.lhead) h1 h2) /\
+         (~(g_is_singleton h) ==>
+          modifies_2 (non_null h.lhead) (reveal h.nodes).[1] h1 h2) /\
          dlisthead_is_valid h2 y))
 let dlisthead_remove_head #t h =
-  let n = h.lhead in
+  let n = non_null h.lhead in
   if is_singleton h
   then (
     empty_list
   ) else (
-    let next = (!n).flink in
+    let next = non_null (!n).flink in
     recall next;
     // unlink them
     !=|> n;
     !<|= next;
-    { lhead = next ; ltail = h.ltail ; nodes = ghost_tail h.nodes }
+    { lhead = of_non_null next ; ltail = h.ltail ; nodes = ghost_tail h.nodes }
   )
 
 #reset-options
@@ -447,43 +410,43 @@ unfold let ghost_unsnoc (#t:Type) (s:erased (seq t){Seq.length (reveal s) > 0}) 
   let l = length x - 1 in
   hide (slice x 0 l)
 
-#set-options "--z3rlimit 300"
+#set-options "--z3rlimit 50"
 
 val dlisthead_remove_tail: #t:eqtype -> h:nonempty_dlisthead t ->
   ST (dlisthead t)
     (requires (fun h0 -> dlisthead_is_valid h0 h))
     (ensures (fun h1 y h2 ->
-         (is_singleton h ==>
-          modifies_1 (getSome h.ltail) h1 h2) /\
-         (~(is_singleton h) ==>
+         (g_is_singleton h ==>
+          modifies_1 (non_null h.ltail) h1 h2) /\
+         (~(g_is_singleton h) ==>
           (let nodes = reveal h.nodes in
-          modifies_2 (getSome h.ltail) nodes.[length nodes - 2] h1 h2)) /\
+          modifies_2 (non_null h.ltail) nodes.[length nodes - 2] h1 h2)) /\
          dlisthead_is_valid h2 y))
 let dlisthead_remove_tail #t h =
   if is_singleton h then (
     empty_list
   ) else (
-    let n = h.ltail in
-    let prev = (!n).blink in
+    let n = non_null h.ltail in
+    let prev = non_null (!n).blink in
     recall prev;
     //unlink them
     !<|= n;
     !=|> prev;
-    { lhead = h.lhead ; ltail = prev ; nodes = ghost_unsnoc h.nodes }
+    { lhead = h.lhead ; ltail = of_non_null prev ; nodes = ghost_unsnoc h.nodes }
   )
 
 #reset-options
 
-let rec get_ref_index (#t:Type) (s:seq (gpointer t)) (x:gpointer t{s `contains_by_addr` x}) :
-  GTot (i:nat{i < Seq.length s})
-    (decreases (Seq.length s)) =
-  contains_elim s x;
-  let h, t = Seq.head s, Seq.tail s in
-  if ptr_eq h x then 0 else (
-    contains_cons h t x;
-    1 + get_ref_index t x)
+// let rec get_ref_index (#t:Type) (s:seq (ref t)) (x:ref t{s `contains_by_addr` x}) :
+//   GTot (i:nat{i < Seq.length s})
+//     (decreases (Seq.length s)) =
+//   contains_elim s x;
+//   let h, t = Seq.head s, Seq.tail s in
+//   if compare_addrs h x then 0 else (
+//     contains_cons h t x;
+//     1 + get_ref_index t x)
 
-// val lemma_get_ref_index : #t:Type -> s:seq (gpointer t) -> x:gpointer t{s `contains_by_addr` x} ->
+// val lemma_get_ref_index : #t:Type -> s:seq (ref t) -> x:ref t{s `contains_by_addr` x} ->
 //   Lemma (ensures (
 //     g_ptr_eq s.[get_ref_index s x] x))
 //     (decreases (Seq.length s))
@@ -491,12 +454,12 @@ let rec get_ref_index (#t:Type) (s:seq (gpointer t)) (x:gpointer t{s `contains_b
 // let rec lemma_get_ref_index #t s x =
 //   contains_elim s x;
 //   let h, t = Seq.head s, Seq.tail s in
-//   if ptr_eq h x then () else (
+//   if compare_addrs h x then () else (
 //     contains_cons h t x;
 //     lemma_get_ref_index t x)
 
-// val split_seq_at_element : #t:Type -> s:seq (gpointer t) -> x:gpointer t{s `contains_by_addr` x} ->
-//   GTot (v:(seq (gpointer t) * nat * seq (gpointer t)){
+// val split_seq_at_element : #t:Type -> s:seq (ref t) -> x:ref t{s `contains_by_addr` x} ->
+//   GTot (v:(seq (ref t) * nat * seq (ref t)){
 //       let l, i, r = v in
 //       indexable s i /\ (
 //       let (i:nat{i < length s}) = i in // workaround for two phase thing
@@ -520,12 +483,12 @@ val dlisthead_remove_strictly_mid: #t:eqtype -> h:nonempty_dlisthead t -> e:gpoi
          is_not_null (e@h1).flink /\ is_not_null (e@h1).blink /\
          dlist_is_valid h2 e /\
          is_null (e@h2).flink /\ is_null (e@h2).blink /\
-         modifies_3 e (getSome (e@h1).flink) (getSome (e@h1).blink) h1 h2 /\
+         modifies_3 e (non_null (e@h1).flink) (non_null (e@h1).blink) h1 h2 /\
          dlisthead_is_valid h2 y))
 let dlisthead_remove_strictly_mid #t h e =
   let h1 = ST.get () in
-  let prev = (!e).blink in
-  let next = (!e).flink in
+  let prev = non_null (!e).blink in
+  let next = non_null (!e).flink in
   lemma_all_elements_distinct (ST.get ()) h; // required to be able to say [prev]
                                              //     and [next] are not same
   recall prev;
